Fix semtyping

proofs/theories/normalform.v
@@ -92,12 +92,19 @@ Proof. sfirstorder use:ne_nf. Qed.
 Lemma nf_wn v : nf v -> wn v.
 Proof. sfirstorder ctrs:rtc. Qed.
 
-(* (* natural number values are normal *) *)
-(* Lemma nat_val_nf v : is_nat_val v -> nf v. *)
-(* Proof. elim : v =>//=. Qed. *)
+Function is_nat_val (a : tm) : bool :=
+  match a with
+  | tZero => true
+  | tSuc a => is_nat_val a
+  | _ => ne a
+end.
 
-(* Lemma ne_nat_val v : ne v -> is_nat_val v. *)
-(* Proof. elim : v =>//=. Qed. *)
+(* natural number values are normal *)
+Lemma nat_val_nf v : is_nat_val v -> nf v.
+Proof. elim : v =>//=. Qed.
+
+Lemma ne_nat_val v : ne v -> is_nat_val v.
+Proof. elim : v =>//=. Qed.
 
 (* Neutral and normal forms are stable under renaming *)
 Lemma ne_nf_renaming (a : tm) :
@@ -125,7 +132,7 @@ Lemma ne_preservation : forall a b, (a ⇒ b) -> ne a -> ne b.
 Proof. sfirstorder use:nf_ne_preservation b:on. Qed.
 
 Create HintDb nfne.
-#[export]Hint Resolve (* ne_nat_val *) nf_wn (* nat_val_nf *) ne_nf wne_wn ne_preservation nf_preservation : nfne.
+#[export]Hint Resolve ne_nat_val nf_wn nat_val_nf ne_nf wne_wn ne_preservation nf_preservation : nfne.
 
 
 (* ------------------ antirenaming ------------------------- *)
