proofs/theories/semtyping.v
@@ -41,6 +41,7 @@ Definition SumSpace Ξ ℓ0 (PA : T -> tm -> Prop) (PF : tm -> (T -> tm -> Prop)
 Reserved Notation " ⟦ Ξ ⊨ A ⟧ i ; I ↘ S" (at level 70, no associativity).
 Inductive InterpExt Ξ i (I : nat -> tm -> Prop) : tm -> (T -> tm -> Prop) -> Prop :=
 | InterpExt_Ne A : ne A -> ⟦ Ξ ⊨ A ⟧ i ; I ↘ (fun ℓ a => IOk Ξ ℓ a /\ wne a)
+| InterpExt_Nat : ⟦ Ξ ⊨ tNat ⟧ i ; I ↘ (fun ℓ a => IOk Ξ ℓ a /\ exists v, a ⇒* v /\ is_nat_val v)
 | InterpExt_Fun ℓ0 A B PA PF :
   InterpExt Ξ i I A PA ->
   (forall a, PA ℓ0 a -> exists PB, PF a PB) ->
@@ -109,7 +110,7 @@ Lemma InterpExt_lt_redundant i Ξ I A PA
 Proof.
   elim : A PA / h.
   - hauto lq:on ctrs:InterpExt.
-  (* - hauto l:on. *)
+  - hauto l:on.
   - hauto l:on ctrs:InterpExt.
   - move => m h.
     apply InterpExt_Univ' => //.
@@ -130,7 +131,7 @@ Lemma InterpExt_lt_redundant2 Ξ i I A PA
 Proof.
   elim : A PA / h.
   - hauto lq:on ctrs:InterpExt.
-  (* - hauto l:on. *)
+  - hauto l:on.
   - hauto l:on ctrs:InterpExt.
   - move => m ?.
     apply InterpExt_Univ' => //.
@@ -247,7 +248,7 @@ Proof.
   move : B.
   elim : A P / h; auto.
   - hauto lq:on ctrs:InterpExt db:nfne.
-  (* - hauto lq:on inv:Par ctrs:InterpExt. *)
+  - hauto lq:on inv:Par ctrs:InterpExt.
   - move => ℓ0 A B PA PF hPA ihPA hPB hPB' ihPB T hT.
     elim /Par_inv :  hT => //.
     move => hPar ℓ1 A0 A1 B0 B1 h0 h1 [? ? ?] ?; subst.
@@ -256,20 +257,6 @@ Proof.
     apply : ihPB; eauto.
     sfirstorder use:Par_cong, Par_refl.
   - hauto lq:on inv:Par ctrs:InterpExt.
-  (* - move => a b A  ? ? ? B. *)
-  (*   elim /Par_inv=>// h ? ? ? a0 b0 A0 ? ? ? [] *. subst. *)
-  (*   apply InterpExt_Eq'; eauto with nfne. *)
-  (*   fext => p. *)
-  (*   f_equal. *)
-  (*   apply propositional_extensionality. *)
-  (*   hauto lq:on use:Par_Coherent, Coherent_transitive, Coherent_symmetric. *)
-  (* - move => A B PA PF hPA ihPA hPB hPB' ihPB T hT. *)
-  (*   elim /Par_inv :  hT => //. *)
-  (*   move => hPar A0 A1 B0 B1 h0 h1 [? ?] ?; subst. *)
-  (*   apply InterpExt_Sig; auto. *)
-  (*   move => a PB hPB0. *)
-  (*   apply : ihPB; eauto. *)
-  (*   sfirstorder use:Par_cong, Par_refl. *)
   - inversion 1. sfirstorder.
   - move => ℓ0 a b ? ?  B.
     elim /Par_inv => // _ ℓ1 ? ? a0 b0 ? ?[*]. subst.
@@ -343,14 +330,14 @@ Proof.
   hauto l:on inv:- db:nfne.
 Qed.
 
-(* Lemma InterpExt_Nat_inv i I P : *)
-(*   ⟦ tNat ⟧ i , I ↘ P -> *)
-(*   P = fun a => exists v, a ⇒* v /\ is_nat_val v. *)
-(* Proof. *)
-(*   move E : tNat => A h. *)
-(*   move : E. *)
-(*   elim : A P / h; hauto q:on inv:tm,Par. *)
-(* Qed. *)
+Lemma InterpExt_Nat_inv Ξ i I P :
+  ⟦ Ξ ⊨ tNat ⟧ i ; I ↘ P ->
+  P = fun ℓ a => IOk Ξ ℓ a /\ exists v, a ⇒* v /\ is_nat_val v.
+Proof.
+  move E : tNat => A h.
+  move : E.
+  elim : A P / h; hauto q:on inv:tm,Par.
+Qed.
 
 Lemma InterpExt_Univ_inv Ξ i I P j :
   ⟦ Ξ ⊨ tUniv j ⟧ i ; I ↘ P ->
@@ -422,38 +409,10 @@ Proof.
   sfirstorder use:InterpExt_Ne_inv rew:db:InterpUniv.
 Qed.
 
-(* Lemma InterpUnivN_Nat_inv i P : *)
-(*   ⟦ tNat ⟧ i ↘ P -> *)
-(*   P = fun a => exists v, a ⇒* v /\ (is_nat_val v). *)
-(* Proof. hauto l:on rew:db:InterpUnivN use:InterpExt_Nat_inv. Qed. *)
-
-(* Lemma InterpExt_Eq_inv i I a b A P : *)
-(*   ⟦ tEq a b A ⟧ i , I ↘ P -> *)
-(*   (P = fun A => A ⇒* tRefl /\ Coherent a b \/ wne A) /\ wn a /\ wn b /\ wn A. *)
-(* Proof. *)
-(*   move E : (tEq a b A) => T h. *)
-(*   move : a b A E. *)
-(*   elim : T P /h => //. *)
-(*   hauto q:on inv:tm. *)
-(*   hauto lq:on ctrs:rtc. *)
-(*   move => A A0 PA hred hA0 ih a b A1 ?. subst. *)
-(*   elim /Par_inv : hred=>//. *)
-(*   move => hred ? ? ? a2 b2 A2 ? ? ? [] *;subst. *)
-(*   split; last by hauto lq:on rew:off ctrs:rtc. *)
-(*   specialize ih with (1 := eq_refl). *)
-(*   move : ih => [->] *. *)
-(*   fext => A. do 2 f_equal. *)
-(*   apply propositional_extensionality. *)
-(*   hauto lq:on use:Par_Coherent, Coherent_symmetric, Coherent_transitive. *)
-(* Qed. *)
-
-(* Lemma InterpUnivN_Eq_inv i a b A P : *)
-(*   ⟦ tEq a b A ⟧ i ↘ P -> *)
-(*   P = (fun p => (p ⇒* tRefl /\ Coherent a b) \/ wne p) /\ wn a /\ wn b /\ wn A. *)
-(* Proof. *)
-(*   simp InterpUniv. *)
-(*   hauto l:on use:InterpExt_Eq_inv. *)
-(* Qed. *)
+Lemma InterpUnivN_Nat_inv Ξ i P :
+  ⟦ Ξ ⊨ tNat ⟧ i ↘ P ->
+  P = fun ℓ a => IOk Ξ ℓ a /\ exists v, a ⇒* v /\ (is_nat_val v).
+Proof. hauto l:on rew:db:InterpUnivN use:InterpExt_Nat_inv. Qed.
 
 (* ------------- relation is deterministic ---------------- *)
 
@@ -466,7 +425,7 @@ Proof.
   move : PB.
   elim : A PA / h.
   - hauto lq:on inv:InterpExt ctrs:InterpExt use:InterpExt_Ne_inv.
-  (* - hauto lq:on inv:InterpExt use:InterpExt_Nat_inv. *)
+  - hauto lq:on inv:InterpExt use:InterpExt_Nat_inv.
   - move => ℓ0 A B PA PF hPA ihPA hPB hPB' ihPB P hP.
     move /InterpExt_Fun_inv : hP.
     intros (PA0 & PF0 & hPA0 & hPB0 & hPB0' & ?); subst.
@@ -525,6 +484,7 @@ Proof.
   elim : A PA / h.
   - sfirstorder.
   - hauto lq:on.
+  - hauto lq:on.
   - sfirstorder.
   - sfirstorder.
   - sfirstorder.
@@ -554,6 +514,7 @@ Proof.
   set tD := tAbsurd (var_tm 0).
   rewrite /CR.
   elim : A PA / h.
+  - firstorder with nfne.
   - firstorder with nfne.
   - move => ℓ0 A B PA PF hPA ihPA hTot hRes ihPF.
     have hzero : PA ℓ0 tD by hauto l:on use:wne_var.
@@ -633,6 +594,7 @@ Proof.
   - hauto q:on inv:IEq.
   - hauto q:on inv:IEq.
   - hauto q:on inv:IEq.
+  - hauto q:on inv:IEq.
   - move => A A0 PA hr hPA ih ℓ B hB hBA.
     move /ifacts.ieq_sym in hBA.
     move : (proj1 (simulation Ξ ℓ)) hBA (hr). repeat move/[apply].
@@ -694,6 +656,7 @@ Lemma InterpExt_IEq Ξ i I A PA  (h : InterpExt Ξ i I A PA) :
 Proof.
   elim : A PA / h.
   - hauto lq:on use:InterpExt_Ne_inv'.
+  - hauto q:on inv:IEq ctrs:InterpExt use:InterpExt_Nat_inv.
   - move => ℓ0 A B PA PF hPA ihPA hTot hRes ihPF ℓ1 T PB.
     elim /IEq_inv=>// _ ? A0 A1 B0 B1 h0 h1 [? ? ?]?. subst.
     move /InterpExt_Fun_inv_nopf.
@@ -779,100 +742,6 @@ Proof.
   hauto q:on rew:db:InterpUniv use:InterpExt_Univ_inv.
 Qed.
 
-(* Lemma InterpUniv_ind (P : nat -> tm -> (tm -> Prop) -> Prop) : *)
-(*   (* Ne *) *)
-(*   (forall i A, ne A -> P i A wne) -> *)
-(*   (* Nat *) *)
-(*   (forall i, P i tNat (fun a : tm => exists v : tm, a ⇒* v /\ is_nat_val v)) -> *)
-(*   (* Pi *) *)
-(*   (forall i A B PA, *)
-(*       ⟦ A ⟧ i ↘ PA -> *)
-(*       P i A PA -> *)
-(*       (forall a, PA a -> exists PB, ⟦ B[a..] ⟧ i ↘ PB /\ P i (B[a..]) PB) -> *)
-(*       (forall a, PA a -> forall PB, ⟦ B[a..] ⟧ i ↘ PB -> P i (B[a..]) PB) -> *)
-(*       P i (tPi A B) (ProdSpace PA (fun a PB => ⟦ B[a..] ⟧ i ↘ PB))) -> *)
-(*   (* Univ *) *)
-(*   (forall i j : fin, j < i -> (forall k A PA, k < i -> ⟦ A ⟧ k ↘ PA -> P k A PA) -> *)
-(*               P i (tUniv j) (fun A => exists PA, ⟦ A ⟧ j ↘ PA)) -> *)
-(*   (* Eq *) *)
-(*   (forall i a b A, *)
-(*       nf a -> *)
-(*       nf b -> nf A -> P i (tEq a b A) (fun p : tm => p ⇒* tRefl /\ a ⇔ b \/ wne p)) -> *)
-(*   (* Sig *) *)
-(*   (forall i A B PA, *)
-(*       ⟦ A ⟧ i ↘ PA -> *)
-(*       P i A PA -> *)
-(*       (forall a, PA a -> exists PB, ⟦ B[a..] ⟧ i ↘ PB /\ P i (B[a..]) PB) -> *)
-(*       (forall a, PA a -> forall PB, ⟦ B[a..] ⟧ i ↘ PB -> P i (B[a..]) PB) -> *)
-(*       P i (tSig A B) (SumSpace PA (fun a PB => ⟦ B[a..] ⟧ i ↘ PB))) -> *)
-(*   (* Red *) *)
-(*   (forall i A A0 PA, *)
-(*       A ⇒ A0 -> ⟦ A0 ⟧ i ↘ PA -> P i A0 PA -> P i A PA) -> *)
-(*   forall i A S, ⟦ A ⟧ i ↘ S -> P i A S. *)
-(* Proof. *)
-(*   move => hNe hNat hFun hUniv hEq hSig hStep. *)
-(*   elim /Wf_nat.lt_wf_ind => i ihOM A S h. *)
-(*   simp InterpUniv in h. *)
-(*   elim : A S / h; eauto. *)
-(*   - repeat rewrite <- InterpUnivN_nolt in *. *)
-(*     move => A B PA PF hPA ihPA hTot hPF ihPF. *)
-(*     have <- : (ProdSpace PA (fun (a : tm) (PB : tm -> Prop) => ⟦ B[a..] ⟧ i ↘ PB)) = ProdSpace PA PF. *)
-(*     rewrite /ProdSpace. *)
-(*     fext => b a PB ha. *)
-(*     apply propositional_extensionality. *)
-(*     split. *)
-(*     hauto l:on. *)
-(*     move => h hPB. *)
-(*     move /hTot : ha => [PB0 /[dup] ? /hPF]. *)
-(*     have ? : PB0 = PB by eauto using InterpUnivN_deterministic. subst. *)
-(*     tauto. *)
-
-(*     apply hFun; auto. *)
-(*     hauto lq:on. *)
-(*     move => a /[dup] ha /hTot. move => [PB hPB]. *)
-(*     move /hPF : (hPB). move => ? PB0 *. *)
-(*     suff : PB = PB0 by hauto lq:on. *)
-(*     eauto using InterpUnivN_deterministic. *)
-(*   - move => A B PA PF hPA ihPA hTot hPF ihPF. *)
-(*     rewrite -InterpUnivN_nolt in hPF ihPF hPA. *)
-(*     have <- : (SumSpace PA (fun (a : tm) (PB : tm -> Prop) => ⟦ B[a..] ⟧ i ↘ PB)) = SumSpace PA PF. *)
-
-(*     rewrite /SumSpace. fext => t. *)
-(*     apply propositional_extensionality. *)
-(*     split. *)
-(*     case; last by tauto. *)
-(*     hauto lq:on. *)
-(*     case; last by tauto. *)
-(*     move => [a][b][h0][h1]h2. left. *)
-(*     exists a,b. *)
-(*     (repeat split) =>// PB hPB. *)
-(*     move /hTot : (h1) => [PB0 /[dup] ? /hPF ?]. *)
-(*     have -> : PB = PB0 by eauto using InterpUnivN_deterministic. *)
-(*     by firstorder. *)
-
-(*     apply hSig; eauto. *)
-(*     hauto lq:on. *)
-(*     move => a ha PB ?. *)
-(*     move /hTot  : (ha) => [PB0 /[dup] /hPF] *. *)
-(*     have -> : PB = PB0 by eauto using InterpUnivN_deterministic. *)
-(*     hauto l:on. *)
-(*   - rewrite -!InterpUnivN_nolt. *)
-(*     sfirstorder. *)
-(* Qed. *)
-
-(* ---- Alternative intro rule for Eq ----------- *)
-(* Lemma InterpUnivN_Eq i a b A: *)
-(*   wn a -> wn b -> wn A -> *)
-(*   ⟦ tEq a b A ⟧ i ↘ (fun p => (p ⇒* tRefl /\ Coherent a b) \/ wne p). *)
-(* Proof. *)
-(*   move => [va [? ?]] [vb [? ?]] [vA [? ?]]. *)
-(*   have ? : InterpUnivN i (tEq va vb vA) (fun p => (p ⇒* tRefl /\ Coherent va vb) \/ wne p) *)
-(*     by hauto lq:on ctrs:InterpExt rew:db:InterpUniv. *)
-(*   have ? : (tEq a b A) ⇒* (tEq va vb vA) by auto using S_Eq. *)
-(*   have : InterpUnivN i (tEq a b A) (fun p => (p ⇒* tRefl /\ Coherent va vb) \/ wne p) by eauto using InterpUnivN_back_preservation_star. *)
-(*   move /[dup] /InterpUnivN_Eq_inv. move => [?]. congruence. *)
-(* Qed. *)
-
 Lemma InterpUnivN_Univ Ξ i j :
   j < i ->
   ⟦ Ξ ⊨ tUniv j ⟧ i ↘  (fun ℓ A => IOk Ξ ℓ A /\ exists PA, InterpUnivN Ξ j A PA).
@@ -899,6 +768,7 @@ Lemma InterpExt_back_clos Ξ i I A PA (hI : forall i A B, I i A -> B ⇒ A -> I 
 Proof.
   move => h.
   elim : A PA / h.
+  - hauto lq:on ctrs:rtc.
   - hauto lq:on ctrs:rtc.
   - have ? : forall ℓ0 b0 b1 a, b0 ⇒ b1 -> tApp b0 ℓ0 a ⇒ tApp b1 ℓ0 a
         by hauto lq:on ctrs:Par use:Par_refl.
@@ -938,173 +808,7 @@ Qed.
 
 (* (* ------------------------ adequacy ------------------------------- *) *)
 
-(* (* P identifies a set of "reducibility candidates" *) *)
-(* Definition CR (P : tm -> Prop) := *)
-(*   (forall a, P a -> wn a) /\ *)
-(*     (forall a, wne a -> P a). *)
-
-(* (* Every interpretation of types is a reducibility candidate *) *)
-(* Lemma adequacy i A PA *)
-(*   (h :  ⟦ A ⟧ i ↘ PA) : *)
-(*   CR PA /\ wn A. *)
-(* Proof. *)
-(*   move : i A PA h. *)
-(*   apply InterpUniv_ind. *)
-(*   - firstorder with nfne. *)
-(*   - hauto lq:on db:nfne. *)
-(*   - move => i A B PA hPA ihPA hPB ihPB. *)
-(*     have hzero : PA (var_tm var_zero) by hauto lq:on ctrs:rtc. *)
-(*     repeat split. *)
-(*     + rewrite /ProdSpace => b hb. *)
-(*       move /hPB : (hzero) => [PB][ih0]ih1. *)
-(*       apply ext_wn with (i := var_zero). hauto lq:on. *)
-(*     + rewrite /ProdSpace => b hb a PB ha. *)
-(*       suff : wn a by hauto q:on use:wne_app. hauto q:on. *)
-(*     + apply wn_pi. *)
-(*       sfirstorder. *)
-(*       move /hPB : (hzero). *)
-(*       move => [_][_][_]h. *)
-(*       apply wn_antirenaming with (ξ := (0..)). *)
-(*       move : h. substify. by asimpl. *)
-(*   - move => m i hlt ih. *)
-(*     repeat split. *)
-(*     + sfirstorder. *)
-(*     + hauto lq:on use:InterpUnivN_WNe. *)
-(*     + hauto lq:on ctrs:rtc. *)
-(*   - hauto lq:on use:wn_eq ctrs:rtc db:nfne. *)
-(*   - move => i A B PA hPA [[ihA0 ihA1] ihA2] ihPB ihPB'. *)
-(*     rewrite /SumSpace. *)
-(*     repeat split. *)
-(*     + move => t []; last by apply wne_wn. *)
-(*       move => [a][b][h0 [h1 h2]]. *)
-(*       rewrite /wn. *)
-(*       suff : wn (tPack a b) by qauto l:on use:rtc_transitive. *)
-(*       have : wn b by hauto q:on. *)
-(*       have : wn a by sfirstorder. *)
-(*       apply wn_pack. *)
-(*     + tauto. *)
-(*     + apply wn_sig; first by auto. *)
-(*       have /ihPB : PA (var_tm 0) by hauto q:on ctrs:rtc. *)
-(*       set q := (X in wn X). *)
-(*       move => ?. have : wn q by sfirstorder. *)
-(*       have -> : q = B⟨0..⟩. *)
-(*       subst q. substify; by asimpl. *)
-(*       apply wn_antirenaming. *)
-(*   - hauto lq:on ctrs:rtc unfold:CR. *)
-(* Qed. *)
-
-(* Corollary InterpUniv_wn_ty i A PA *)
-(*   (h : ⟦ A ⟧ i ↘ PA) : *)
-(*   wn A. *)
-(* Proof. firstorder using adequacy. Qed. *)
-
-(* Derive Inversion sub1_inv with (forall A B, Sub1 A B). *)
-
-(* Lemma Sub1_ne A B : Sub1 A B -> ne A = ne B /\ nf A = nf B. *)
-(* Proof. elim; sfirstorder. Qed. *)
-
-(* Lemma InterpUnivN_Sub1 : forall i  A PA, *)
-(*    ⟦ A ⟧ i  ↘ PA ->  forall j B PB, ⟦ B ⟧ j  ↘ PB -> *)
-(*   (Sub1 A B -> *)
-(*   forall a, PA a -> PB a) /\ (Sub1 B A -> forall a, PB a -> PA a). *)
-(* Proof. *)
-(*   apply : InterpUniv_ind. *)
-(*   - move => _ A h j B PB hPB. *)
-(*     split => ?; *)
-(*       (have : ne B by hauto l:on use:Sub1_ne inv:Sub1); *)
-(*       hauto lq:on rew:off inv:Sub1 use:InterpUnivN_Ne_inv. *)
-(*   - move => _ j B PB hB. *)
-(*     split;inversion 1; subst; move/InterpUnivN_Nat_inv in hB; *)
-(*       sfirstorder. *)
-(*   - move => i A0 B0 PA0 hPA0 ihA0 hTot ihPF j B PB hPB. *)
-(*     have ? : ⟦ tPi A0 B0 ⟧ i ↘ (ProdSpace PA0 (fun (a0 : tm) (PB0 : tm -> Prop) => ⟦ B0[a0..] ⟧ i ↘ PB0)) by hauto l:on use:InterpUnivN_Fun_nopf. *)
-(*     split. *)
-(*     + elim /sub1_inv=>//. *)
-(*       move => _ A1 B1 A2 B2 hs1 hs2 []? ? ?. subst. *)
-(*       move /InterpUnivN_Fun_inv_nopf : hPB => [PA1][hPA1][hTot']?. subst. *)
-(*       have {}ihA0 : forall a, PA1 a -> PA0 a by hauto l:on. *)
-(*       move => b hb a PB2 ha hPB2. *)
-(*       have [ PB0 hPB0 ] : exists PB, ⟦ B0[a..] ⟧ i  ↘ PB *)
-(*         by qauto l:on. *)
-(*       have : Sub1 B0[a..] B2[a..] by sfirstorder use:Sub1_morphing. *)
-(*       rewrite /ProdSpace in hb. *)
-(*       move /ihPF : hPB2 (hPB0). move/[apply]. *)
-(*       hauto lq:on unfold:ProdSpace. *)
-(*     + elim /sub1_inv=>//. *)
-(*       move => _ A1 B1 A2 B2 hs1 hs2 ?[] ? ?. subst. *)
-(*       move /InterpUnivN_Fun_inv_nopf : hPB => [PA1][hPA1][hTot']?. subst. *)
-(*       have {}ihA0 : forall a, PA0 a -> PA1 a by hauto l:on. *)
-(*       move => b hb a PB0 ha hPB0. *)
-(*       have ? : Sub1 B1[a..] B0[a..] by sfirstorder use:Sub1_morphing. *)
-(*       move /ihPF : hPB0 {ihPF}. *)
-(*       move /(_ _ ltac:(sfirstorder)) : hTot'  => [PB1 hPB1]. *)
-(*       move => h. eapply h; eauto. *)
-(*       sfirstorder. *)
-(*   - move => j j0 ? ? j1 B PB hPB. *)
-(*     split. *)
-(*     + elim /sub1_inv=>//. *)
-(*       move => _ p q ? []? ? a ha. subst. *)
-(*       move /InterpUnivN_Univ_inv  : hPB. *)
-(*       hauto l:on use:InterpUnivN_cumulative. *)
-(*     + elim /sub1_inv=>//. *)
-(*       move => _ p q ? ? [?] a ha. subst. *)
-(*       move /InterpUnivN_Univ_inv  : hPB. *)
-(*       move => [? ?]. subst. *)
-(*       hauto l:on use:InterpUnivN_cumulative. *)
-(*   - move => i  > h0 h1 h2 > h. *)
-(*     split; inversion 1; subst; *)
-(*       move /InterpUnivN_Eq_inv : h => [? ?]; subst; auto. *)
-(*   - move => i A0 B0 PA0 hPA0 ihPA0 hPF ihPF j B PB hPB. *)
-(*     have ? : ⟦ tSig A0 B0 ⟧ i ↘ (SumSpace PA0 (fun (a0 : tm) (PB0 : tm -> Prop) => ⟦ B0[a0..] ⟧ i ↘ PB0)) by hauto l:on use:InterpUnivN_Sig_nopf. *)
-(*     split. *)
-(*     + elim /sub1_inv=>//. *)
-(*       move => _ A1 B1 A2 B2 hs1 hs2 []? ? ?. subst. *)
-(*       move /InterpUnivN_Sig_inv_nopf : hPB => [PA1][hPA1][hTot']?. subst. *)
-(*       have {}ihA0 : forall a, PA0 a -> PA1 a by hauto l:on. *)
-(*       move => t. rewrite /SumSpace. *)
-(*       move => []; last by tauto. *)
-(*       move => [a][b][h0][h1]h2. *)
-(*       left. exists a,b. (repeat split) => //. by firstorder. *)
-(*       move => PB hPB. *)
-(*       have [ PB0 hPB0 ] : (exists PB, ⟦ B0[a..] ⟧ i  ↘ PB) *)
-(*         by qauto l:on. *)
-(*       have : Sub1 B0[a..] B2[a..] by sfirstorder use:Sub1_morphing. *)
-(*       qauto l:on. *)
-(*     + elim /sub1_inv=>//. *)
-(*       move => _ A1 B1 A2 B2 hs1 hs2 ? [? ?] t. subst. *)
-(*       move /InterpUnivN_Sig_inv_nopf : hPB => [PA1][hPA1][hTot']?. subst. *)
-(*       have {}ihA0 : forall a, PA1 a -> PA0 a by hauto l:on. *)
-(*       rewrite /SumSpace. move => []; last by tauto. *)
-(*       qauto l:on use:Sub1_morphing. *)
-(*   - move => i A A0 PA hred hPA ih j B PB hPB. *)
-(*     split. *)
-(*     + move => hSub a ha. *)
-(*       have : exists B0, B ⇒ B0 /\ Sub1 A0 B0 by qauto l:on use:Sub1_simulation. *)
-(*       move => [B0][h0]h1. *)
-(*       have /ih : ⟦ B0 ⟧ j ↘ PB by eauto using InterpUnivN_preservation. *)
-(*       sfirstorder. *)
-(*     + move => hSub a ha. *)
-(*       have : exists B0, B ⇒ B0 /\ Sub1 B0 A0 by qauto l:on use:Sub1_simulation. *)
-(*       move => [B0][h0]h1. *)
-(*       have /ih : ⟦ B0 ⟧ j ↘ PB by eauto using InterpUnivN_preservation. *)
-(*       sfirstorder. *)
-(* Qed. *)
-
-(* Lemma InterpUnivN_Sub1' i j A B PA PB (h : ⟦ A ⟧ i ↘ PA) (h2 : ⟦ B ⟧ j ↘ PB) : *)
-(*   (Sub1 A B -> forall a, PA a -> PB a). *)
-(* Proof. hauto l:on use:InterpUnivN_Sub1. Qed. *)
-
-(* Lemma InterpUnivN_Sub i j A B PA PB (h0 : ⟦ A ⟧ i ↘ PA) (h1 : ⟦ B ⟧ j ↘ PB) (h2 : Sub A B) : *)
-(*   forall a, PA a -> PB a. *)
-(* Proof. *)
-(*   move : h2. rewrite /Sub. *)
-(*   move => [A0][B0][h2][h3]+. *)
-(*   have : ⟦ B0 ⟧ j ↘ PB by hauto lq:on use:InterpUnivN_Coherent ctrs:rtc. *)
-(*   have : ⟦ A0 ⟧ i ↘ PA by hauto lq:on use:InterpUnivN_Coherent ctrs:rtc. *)
-(*   apply InterpUnivN_Sub1'. *)
-(* Qed. *)
-
-(* Lemma InterpUnivN_Nat : ⟦ tNat ⟧ 0 ↘ (fun a => exists v, a ⇒* v /\ is_nat_val v). *)
-(* Proof. simp InterpUniv. apply InterpExt_Nat. Qed. *)
+Lemma InterpUnivN_Nat Ξ : ⟦ Ξ ⊨ tNat ⟧ 0 ↘ (fun ℓ a => IOk Ξ ℓ a /\ exists v, a ⇒* v /\ is_nat_val v).
+Proof. simp InterpUniv. apply InterpExt_Nat. Qed.
 
 End lr_sig.
